src/examples/Kuiper.Example.Array1.fst
@@ -1,0 +1,47 @@
+module Kuiper.Example.Array1
+
+#lang-pulse
+open Kuiper
+open Kuiper.Array1
+module Array1 = Kuiper.Array1
+open Kuiper.Injection
+module SZ = Kuiper.SizeT
+
+let layout (m : nat) : layout m = {
+  ulen = m;
+  imap = mk_injection (fun i -> i) ez;
+}
+
+inline_for_extraction noextract
+instance blah (m : SZ.t{SZ.fits m}) : clayout (layout m) =
+  {
+    culen = m;
+    all_fit = ();
+    cimap = (fun i -> i);
+  }
+
+fn test0 (m : array1 u32 (layout 10))
+{
+  ()
+}
+
+// Should not be needed, maybe Kuiper.concrete can solve this eventually
+inline_for_extraction noextract
+instance _crutch : clayout (layout 100) = blah 100sz
+
+fn test1 (m : array1 u32 (layout 100))
+  preserves m |-> 's
+  returns u32
+{
+  let v = Array1.read m 1sz;
+  v
+}
+
+fn test2 (m : array1 u32 (layout 100))
+  requires m |-> 's
+  // ensures  m |-> Kuiper.Chest.upd 's ((1 <: natlt 10), ((2 <: natlt 20), ())) 42ul
+  ensures  m |-> Kuiper.Seq.Common.lseq_upd 's (1 <: natlt 100) 42ul
+{
+  Array1.write m 1sz 42ul;
+  ()
+}
