src/lib/data/Kuiper.Array1.fst
@@ -1,0 +1,246 @@
+module Kuiper.Array1
+#lang-pulse
+
+open Kuiper
+open Kuiper.Chest
+open Kuiper.Bijection
+module T = Kuiper.Tensor
+module SZ = Kuiper.SizeT
+module Tac = FStar.Tactics.V2
+
+let tr_layout (#len : nat) (l : layout len) : tlayout (ICons len INil) = {
+  ulen = l.ulen;
+  imap = mk_injection (fun (i, ()) -> l.imap.f i) ez;
+}
+
+let abs_bij (#len : nat) : (abs (ICons len INil) =~ natlt len) =
+  {
+    ff = (fun (i, ()) -> i);
+    gg = (fun i -> (i, ()));
+    ff_gg = ez;
+    gg_ff = ez;
+  }
+
+let tr_val (#et : Type) (#len : nat) (s : lseq et len) : chest (ICons len INil) et =
+  Chest.mk (ICons len INil) (fun (i, ()) -> s @! i)
+
+inline_for_extraction noextract
+instance clayout_to_tlayout (#len : erased nat) (#l : layout len)
+  (c : clayout l)
+  : ctlayout (tr_layout l) =
+{
+  culen   = c.culen;
+  all_fit = ();
+  cimap   = (fun (idx : conc (ICons len INil)) ->
+              match idx with
+              | (i, ()) -> c.cimap i);
+}
+
+let t (et : Type0) (#len : nat) (l : layout len) : Type0 =
+  T.tensor et (tr_layout l)
+
+let is_global (#et : Type0) (#len : nat) (#l : layout len)
+  (a : t et l)
+  : prop =
+  T.is_global_tensor a
+
+let from_array
+  (#et : Type0) (#len : erased nat)
+  (l : layout len)
+  (a : gpu_array et (layout_size l))
+  : t et l
+  = T.from_array _ a
+
+let core
+  (#et : Type0) (#len : erased nat) (#l : layout len)
+  (a : t et l)
+  : gpu_array et (layout_size l)
+  = T.core a
+
+let lem_core_from_array
+  (#et : Type) (#len : erased nat)
+  (#l : layout len)
+  (a : t et l)
+  : Lemma (ensures from_array l (core a) == a)
+          [SMTPat (core a)]
+   = ()
+
+let lem_from_array_core
+  (#et : Type) (#len : erased nat)
+  (l : layout len)
+  (p : gpu_array et (layout_size l))
+  : Lemma (ensures core (from_array l p) == p)
+          [SMTPat (from_array l p)]
+  = ()
+
+let lem_is_global_iff_core
+  (#et : Type0) (#len : nat)
+  (#l : layout len)
+  (a : t et l)
+  : Lemma (ensures is_global a <==> is_global_array (core a))
+          [SMTPat (is_global a)]
+  = ()
+
+let pts_to
+  (#et : Type) (#len : nat) (#l : layout len)
+  ([@@@mkey] a : t et l)
+  (#[Tac.exact (`1.0R)] f : perm)
+  (s : lseq et len)
+  : slprop
+  = T.tensor_pts_to a #f (tr_val s)
+
+instance is_send_across_global
+  (#et : Type0) (#len : nat) (#l : layout len)
+  (a : t et l { is_global a })
+  (#f : perm) (s : lseq et len)
+  : is_send_across gpu_of (pts_to a #f s)
+  = solve
+
+ghost
+fn pts_to_ref
+  (#et : Type) (#len : nat) (#l : layout len)
+  (a : t et l)
+  (#f : perm) (#s : erased (lseq et len))
+  preserves
+    a |-> Frac f s
+  ensures
+    pure (SZ.fits (layout_size l))
+{
+  unfold pts_to a #f s;
+  T.tensor_pts_to_ref a;
+  fold pts_to a #f s;
+}
+
+ghost
+fn share_n
+  (#et : Type0) (#len : nat) (#l : layout len)
+  (a : t et l) (k : pos)
+  (#f : perm) (#s : lseq et len)
+  requires
+    a |-> Frac f s
+  ensures
+    forall+ (_:natlt k). a |-> Frac (f /. k) s
+{
+  unfold pts_to a #f s;
+  T.tensor_share_n a k;
+  forevery_map
+    (fun (i:natlt k) -> T.tensor_pts_to a #(f /. k) (tr_val s))
+    (fun (i:natlt k) -> pts_to a #(f /. k) s)
+    fn i { fold pts_to a #(f /. k) s };
+}
+
+ghost
+fn gather_n
+  (#et : Type0) (#len : nat) (#l : layout len)
+  (a : t et l) (k : pos)
+  (#f : perm) (#s : lseq et len)
+  requires
+    forall+ (_:natlt k). a |-> Frac (f /. k) s
+  ensures
+    a |-> Frac f s
+{
+  forevery_map
+    (fun (i:natlt k) -> pts_to a #(f /. k) s)
+    (fun (i:natlt k) -> T.tensor_pts_to a #(f /. k) (tr_val s))
+    fn i { unfold pts_to a #(f /. k) s };
+  T.tensor_gather_n a k;
+  fold pts_to a #f s;
+}
+
+inline_for_extraction noextract
+fn read
+  (#et : Type0)
+  (#len : erased nat)
+  (#l : layout len) {| clayout l |}
+  (a : t et l)
+  (i : szlt len)
+  (#f : perm)
+  (#s : erased (lseq et len))
+  preserves
+    a |-> Frac f s
+  returns
+    v : et
+  ensures
+    pure (v == Seq.index s i)
+{
+  unfold pts_to a #f s;
+  let idx = (i, ());
+  let v = T.tensor_read a idx;
+  fold pts_to a #f s;
+  v
+}
+
+inline_for_extraction noextract
+fn write
+  (#et : Type0)
+  (#len : erased nat)
+  (#l : layout len) {| clayout l |}
+  (a : t et l)
+  (i : szlt len)
+  (v : et)
+  (#s : erased (lseq et len))
+  requires a |-> s
+  ensures  a |-> (Seq.upd s i v <: lseq et len)
+{
+  unfold pts_to a s;
+  T.tensor_write a (i, ()) v;
+  with cs'. assert T.tensor_pts_to a cs';
+  assert pure (Chest.equal cs' (tr_val (Seq.upd s i v)));
+  fold pts_to a (Seq.upd s i v);
+  ()
+}
+
+let pts_to_cell
+  (#et : Type) (#len : nat) (#l : layout len)
+  ([@@@mkey] a : t et l)
+  (#[Tac.exact (`1.0R)] f : perm)
+  ([@@@mkey] i : natlt len)
+  (v : et)
+  : slprop
+  = T.tensor_pts_to_cell a #f (i, ()) v
+
+let pts_to_cell_eq
+  (#et : Type) (#len : nat) (#l : layout len)
+  (a : t et l) (i : natlt len) (f : perm) (v : et)
+  : Lemma (pts_to_cell a #f i v
+           ==
+           gpu_pts_to_cell (core a) #f (l.imap.f i) v)
+  = T.tensor_pts_to_cell_eq a (i, ()) f v
+
+ghost
+fn explode
+  (#et : Type0) (#len : nat) (#l : layout len)
+  (a : t et l)
+  (#f : perm)
+  (#s : lseq et len)
+  requires a |-> Frac f s
+  ensures
+    forall+ (i : natlt len).
+      Cell a i |-> Frac f (Seq.index s i)
+{
+  unfold pts_to a #f s;
+  T.tensor_explode a;
+  forevery_iso abs_bij _;
+  forevery_ext _ (fun (i : natlt len) -> Cell a i |-> Frac f (Seq.index s i));
+  ()
+}
+
+ghost
+fn implode
+  (#et : Type0) (#len : nat) (#l : layout len)
+  (a : t et l)
+  (#f : perm)
+  (#s : lseq et len)
+  requires
+    pure (SZ.fits (layout_size l))
+  requires
+    forall+ (i : natlt len).
+      Cell a i |-> Frac f (Seq.index s i)
+  ensures
+    a |-> Frac f s
+{
+  forevery_iso (bij_sym abs_bij) _;
+  forevery_ext _ (fun (i : abs (ICons len INil)) -> Cell a i |-> Frac f (acc (tr_val s) i));
+  T.tensor_implode a;
+  fold pts_to a #f s;
+}
