src/lib/data/Kuiper.Array1.fsti
@@ -1,0 +1,240 @@
+module Kuiper.Array1
+
+#lang-pulse
+
+open Kuiper
+open Kuiper.Tensor
+open Kuiper.Injection
+open Kuiper.Index
+open FStar.Tactics.Typeclasses { no_method }
+module V = Kuiper.View
+module SZ = Kuiper.SizeT
+module Tac = FStar.Tactics.V2
+
+[@@erasable]
+noeq
+type layout (len : nat) = {
+  ulen : nat;
+  imap : (natlt len @~> natlt ulen);
+}
+
+let layout_size (#len : nat) (l : layout len) : GTot nat = l.ulen
+
+inline_for_extraction noextract
+class clayout (#len : erased nat) (l : layout len) = {
+  [@@@no_method]
+  culen : (x:SZ.t { SZ.v x == l.ulen });
+
+  [@@@no_method]
+  all_fit : squash (SZ.fits len);
+
+  [@@@no_method]
+  cimap : i:SZ.t{i < len} -> r:SZ.t{SZ.v r == l.imap.f (SZ.v i)};
+}
+
+let aview (et : Type) (#len : nat) (l : layout len)
+  : V.aview et (lseq et len)
+  = {
+      iview = {
+        len = l.ulen;
+        ait = natlt len;
+        step = { imap = l.imap; };
+      };
+      ctn = solve;
+    }
+
+inline_for_extraction noextract
+val t (et : Type0) (#len : nat) (l : layout len) : Type0
+
+unfold let array1 = t
+
+val is_global (#et : Type0) (#len : nat) (#l : layout len)
+  (a : t et l)
+  : prop
+
+inline_for_extraction noextract
+val from_array
+  (#et : Type0) (#len : erased nat)
+  (l : layout len)
+  (a : gpu_array et (layout_size l))
+  : t et l
+
+inline_for_extraction noextract
+val core
+  (#et : Type0) (#len : erased nat) (#l : layout len)
+  (a : t et l)
+  : gpu_array et (layout_size l)
+
+val lem_core_from_array
+  (#et : Type) (#len : erased nat)
+  (#l : layout len)
+  (a : t et l)
+  : Lemma (ensures from_array l (core a) == a)
+          [SMTPat (core a)]
+
+val lem_from_array_core
+  (#et : Type) (#len : erased nat)
+  (l : layout len)
+  (p : gpu_array et (layout_size l))
+  : Lemma (ensures core (from_array l p) == p)
+          [SMTPat (from_array l p)]
+
+val lem_is_global_iff_core
+  (#et : Type0) (#len : nat)
+  (#l : layout len)
+  (a : t et l)
+  : Lemma (ensures is_global a <==> is_global_array (core a))
+          [SMTPat (is_global a)]
+
+val pts_to
+  (#et : Type) (#len : nat) (#l : layout len)
+  ([@@@mkey] a : t et l)
+  (#[Tac.exact (`1.0R)] f : perm)
+  (s : lseq et len)
+  : slprop
+
+instance
+val is_send_across_global
+  (#et : Type0) (#len : nat) (#l : layout len)
+  (a : t et l { is_global a })
+  (#f : perm) (s : lseq et len)
+  : is_send_across gpu_of (pts_to a #f s)
+
+unfold
+instance has_pts_to_inst (et : Type) (len : erased nat) (l : _)
+  : has_pts_to (t et l) (lseq et len)
+  = { pts_to }
+
+ghost
+fn pts_to_ref
+  (#et : Type) (#len : nat) (#l : layout len)
+  (a : t et l)
+  (#f : perm) (#s : erased (lseq et len))
+  preserves
+    a |-> Frac f s
+  ensures
+    pure (SZ.fits (layout_size l))
+
+ghost
+fn share_n
+  (#et : Type0) (#len : nat) (#l : layout len)
+  (a : t et l) (k : pos)
+  (#f : perm) (#s : lseq et len)
+  requires
+    a |-> Frac f s
+  ensures
+    forall+ (_:natlt k). a |-> Frac (f /. k) s
+
+ghost
+fn gather_n
+  (#et : Type0) (#len : nat) (#l : layout len)
+  (a : t et l) (k : pos)
+  (#f : perm) (#s : lseq et len)
+  requires
+    forall+ (_:natlt k). a |-> Frac (f /. k) s
+  ensures
+    a |-> Frac f s
+
+inline_for_extraction noextract
+let clayout_imap
+  (#len : erased nat)
+  (#l : layout len)
+  (c : clayout l)
+  : szlt len -> szlt l.ulen
+  = fun i -> c.cimap i
+
+inline_for_extraction noextract
+instance cfarray_ciview
+  (et : Type)
+  (#len : erased nat)
+  (l : layout len)
+  (c : clayout l)
+  : Kuiper.IView.ciview (aview et l).iview =
+{
+  clen = c.culen;
+  sch = {
+    cit = szlt len;
+    bij = Kuiper.Bijection.natural;
+  };
+  step = {
+    cimap = mk_cinj (clayout_imap c);
+    compat = ez;
+  };
+}
+
+inline_for_extraction noextract
+fn read
+  (#et : Type0)
+  (#len : erased nat)
+  (#l : layout len) {| clayout l |}
+  (a : t et l)
+  (i : szlt len)
+  (#f : perm)
+  (#s : erased (lseq et len))
+  preserves
+    a |-> Frac f s
+  returns
+    v : et
+  ensures
+    pure (v == Seq.index s i)
+
+inline_for_extraction noextract
+fn write
+  (#et : Type0)
+  (#len : erased nat)
+  (#l : layout len) {| clayout l |}
+  (a : t et l)
+  (i : szlt len)
+  (v : et)
+  (#s : erased (lseq et len))
+  requires
+    a |-> s
+  ensures
+    a |-> (Seq.upd s i v <: lseq et len)
+
+val pts_to_cell
+  (#et : Type) (#len : nat) (#l : layout len)
+  ([@@@mkey] a : t et l)
+  (#[Tac.exact (`1.0R)] f : perm)
+  ([@@@mkey] i : natlt len)
+  (v : et)
+  : slprop
+
+[@@pulse_unfold; FStar.Tactics.Typeclasses.noinst]
+instance cell_pts_to (#et : Type) (#len : nat) (#l : layout len)
+  : has_pts_to (cell (t et l) (natlt len)) et
+= {
+  pts_to = (fun (Cell ar i) #f v -> pts_to_cell ar #f i v);
+}
+
+val pts_to_cell_eq
+  (#et : Type) (#len : nat) (#l : layout len)
+  (a : t et l) (i : natlt len) (f : perm) (v : et)
+  : Lemma (Cell a i |-> Frac f v
+           ==
+           gpu_pts_to_cell (core a) #f (l.imap.f i) v)
+
+ghost
+fn explode
+  (#et : Type0) (#len : nat) (#l : layout len)
+  (a : t et l)
+  (#f : perm)
+  (#s : lseq et len)
+  requires a |-> Frac f s
+  ensures
+    forall+ (i : natlt len).
+      Cell a i |-> Frac f (Seq.index s i)
+
+ghost
+fn implode
+  (#et : Type0) (#len : nat) (#l : layout len)
+  (a : t et l)
+  (#f : perm)
+  (#s : lseq et len)
+  requires
+    pure (SZ.fits (layout_size l))
+  requires
+    forall+ (i : natlt len).
+      Cell a i |-> Frac f (Seq.index s i)
+  ensures
+    a |-> Frac f s
